Blake hash incremental spec equivalence, with lemmas about repeati vs update_multi assumed

specs/lemmas/Spec.Hash.Incremental.fst
@@ -6,9 +6,182 @@ open Spec.Hash.Definitions
 open Spec.Hash.PadFinish
 open Spec.Hash.Lemmas
 
+module B2 = Spec.Blake2
+
 friend Spec.Agile.Hash
 
-#set-options "--max_fuel 0 --max_ifuel 0 --z3rlimit 50"
+#set-options "--max_fuel 0 --max_ifuel 0 --z3rlimit 20"
+
+let rec lemma_update_multi_core_blake
+  (a:hash_alg{is_blake a})
+  (blocks:bytes{Seq.length blocks <= max_input_length a})
+  (nb:nat)
+  (h:words_state a)
+  : Lemma
+    (requires snd h == u64 0 /\ Seq.length blocks == nb * block_length a)
+    (ensures fst (Spec.Agile.Hash.update_multi a h blocks) ==
+             Lib.LoopCombinators.repeati nb (B2.blake2_update1 (to_blake_alg a) 0 blocks) (fst h))
+  = let n = S.length blocks / block_length a in
+    let f = B2.blake2_update1 (to_blake_alg a) 0 blocks in
+    let open Lib.LoopCombinators in
+    if nb = 0 then (
+       admit()
+       // assert (blocks `S.equal` S.empty);
+       // update_multi_zero a h;
+       // eq_repeati0 n f (fst h)
+
+    ) else admit ()
+
+let rec lemma_update_multi_core_blake_snd
+  (a:hash_alg{is_blake a})
+  (blocks:bytes{Seq.length blocks <= maxint U64})
+  (nb:nat)
+  (h:words_state a)
+  : Lemma
+    (requires snd h == u64 0 /\ Seq.length blocks == nb * block_length a)
+    (ensures snd (Spec.Agile.Hash.update_multi a h blocks) == u64 (S.length blocks))
+  = admit()
+
+
+#pop-options
+
+let rec repeati_ext (#a:Type) (n:nat) (f1 f2:(i:nat{i < n} -> a -> a)) (acc0:a) (i:nat{i <= n})
+  : Lemma
+    (requires forall (i:nat{i < n}) (acc:a). f1 i acc == f2 i acc)
+    (ensures Lib.LoopCombinators.repeati i f1 acc0 == Lib.LoopCombinators.repeati i f2 acc0)
+    (decreases i)
+  = let open Lib.LoopCombinators in
+    if i = 0 then (
+      eq_repeati0 n f1 acc0;
+      eq_repeati0 n f2 acc0
+    ) else (
+      unfold_repeati n f1 acc0 (i-1);
+      unfold_repeati n f2 acc0 (i-1);
+      repeati_ext n f1 f2 acc0 (i-1)
+    )
+
+#push-options "--z3rlimit 100"
+
+let lemma_blake2_split
+  (a:hash_alg{is_blake a})
+  (d:bytes{Seq.length d <= max_input_length a})
+  (h:words_state a)
+  : Lemma
+    (let (nb, rem) = B2.split (to_blake_alg a) (Seq.length d) in
+     let blocks = Seq.slice d 0 (nb * block_length a) in
+     Lib.LoopCombinators.repeati nb (B2.blake2_update1 (to_blake_alg a) 0 d) (fst h) ==
+     Lib.LoopCombinators.repeati nb (B2.blake2_update1 (to_blake_alg a) 0 blocks) (fst h))
+  = let (nb, rem) = B2.split (to_blake_alg a) (Seq.length d) in
+    let blocks = Seq.slice d 0 (nb * block_length a) in
+    let n = S.length blocks / block_length a in
+    let f1 = B2.blake2_update1 (to_blake_alg a) 0 d in
+    let f2 = B2.blake2_update1 (to_blake_alg a) 0 blocks in
+    repeati_ext n f1 f2 (fst h) nb
+
+#pop-options
+
+let lemma_small_last_split (a:hash_alg{is_blake a}) (input:bytes)
+  : Lemma
+    (requires S.length input <= block_length a)
+    (ensures (let bs, l, rem = last_split_blake a input in
+              bs `S.equal` S.empty /\
+              S.equal l (B2.get_last_padded_block (to_blake_alg a) input rem) /\
+              rem == S.length input))
+  = let bs, l, rem = last_split_blake a input in
+    if S.length input = block_length a then ()
+    else FStar.Math.Lemmas.small_div (S.length input) (block_length a)
+
+let update_last_blake_aux (a:hash_alg{is_blake a})
+  (hash:words_state a)
+  (prevlen:nat{prevlen % block_length a = 0})
+  (input:bytes{S.length input + prevlen <= maxint U64}) :
+  Tot (words_state a)
+  = let blocks, last_block, rem = last_split_blake a input in
+    let h' = update_multi a hash blocks in
+    let h_f = Spec.Blake2.blake2_update_block (to_blake_alg a) true (prevlen + S.length input) last_block (fst h') in
+    (h_f, u64 0)
+
+let lemma_update_last_aux (a:hash_alg{is_blake a})
+  (s:words_state a)
+  (prevlen:nat{prevlen % block_length a = 0})
+  (input:bytes{S.length input + prevlen <= maxint U64}) :
+  Lemma
+    (requires v #U64 #SEC (snd s) == prevlen /\
+      // Not necessary, but simplifies proof, and all we need here
+      S.length input <= block_length a)
+    (ensures
+      update_last_blake a s prevlen input == update_last_blake_aux a s prevlen input)
+  = let b, l, r = last_split_blake a input in
+
+    FStar.Math.Lemmas.small_mod (prevlen + S.length input) (pow2 64)
+
+let lemma_last_padded_block (a:hash_alg{is_blake a}) (blocks l:bytes)
+  (rem:nat{rem <= S.length l /\ rem <= block_length a})
+  : Lemma
+    (requires S.length blocks % block_length a == 0 /\ rem == S.length l)
+    (ensures B2.get_last_padded_block (to_blake_alg a) l rem `S.equal`
+             B2.get_last_padded_block (to_blake_alg a) (blocks `S.append` l) rem)
+  = let m = blocks `S.append` l in
+    let last_m = Seq.slice m (S.length m - rem) (S.length m) in
+    assert (last_m `S.equal` l)
+
+let lemma_update_last_blake2
+  (a:hash_alg{is_blake a})
+  (rem:nat)
+  (d:bytes)
+  (s:words_state a)
+  : Lemma
+    (requires rem <= block_length a /\ rem <= S.length d /\ S.length d <= maxint U64 /\
+      (let bs, l = split_blocks a d in
+       rem == S.length l /\ v #U64 #SEC (snd s) == S.length bs)
+    )
+    (ensures
+      (let bs, l = split_blocks a d in
+      B2.blake2_update_last (to_blake_alg a) 0 rem d (fst s) ==
+      fst (update_last_blake a s (S.length bs) l))
+    )
+  = let bs, l = split_blocks a d in
+
+    lemma_small_last_split a l;
+
+    lemma_update_last_aux a s (S.length bs) l;
+
+    let h_ag = B2.blake2_update_last (to_blake_alg a) 0 rem d (fst s) in
+
+    let last_b = B2.get_last_padded_block (to_blake_alg a) d rem in
+    assert (B2.blake2_update_last (to_blake_alg a) 0 rem d (fst s) ==
+      B2.blake2_update_block (to_blake_alg a) true (S.length d) last_b (fst s));
+
+    let blocks, last_block, r = last_split_blake a l in
+    lemma_last_padded_block a bs l rem;
+
+    let s' = update_multi a s blocks in
+
+    update_multi_zero a s
+
+let lemma_hash_incremental_body_blake2
+  (a:hash_alg{is_blake a})
+  (d:bytes{Seq.length d <= maxint U64})
+  (s:words_state a)
+  : Lemma
+    (requires (snd s) == u64 0)
+    (ensures (
+      fst (hash_incremental_body a d s) ==
+      B2.blake2_update_blocks (to_blake_alg a) 0 d (fst s)))
+  = let open Lib.LoopCombinators in
+    let bs, l = split_blocks a d in
+    let (nb, rem) = B2.split (to_blake_alg a) (Seq.length d) in
+    assert (rem == Seq.length l);
+    assert (nb * block_length a + rem == Seq.length d);
+    let blocks = Seq.slice d 0 (nb * block_length a) in
+    let rest = Seq.slice d (nb * block_length a) (Seq.length d) in
+    let s_ag1 = update_multi a s bs in
+    let s_b1 = repeati nb (B2.blake2_update1 (to_blake_alg a) 0 d) (fst s) in
+    lemma_update_multi_core_blake a bs nb s;
+    lemma_update_multi_core_blake_snd a bs nb s;
+    lemma_blake2_split a d s;
+
+    lemma_update_last_blake2 a rem d s_ag1
 
 let blake2_is_hash_incremental
   (a:hash_alg{is_blake a}) (d:bytes{Seq.length d <= max_input_length a})
@@ -16,6 +189,8 @@ let blake2_is_hash_incremental
     (Spec.Blake2.blake2 (to_blake_alg a) d 0 Seq.empty (Spec.Blake2.max_output (to_blake_alg a)) ==
      hash_incremental a d)
   = admit()
+    // TODO: max_input_length should be pow2 64 for both blake
+    //lemma_hash_incremental_body_blake2 a d (init a)
 
 let hash_is_hash_incremental (a: hash_alg) (input: bytes { S.length input <= max_input_length a }):
   Lemma (ensures (S.equal (hash a input) (hash_incremental a input)))
